greedy axiom 1 verifies

dp/6_4.dfy
@@ -9,33 +9,56 @@ module SixFour {
     // Limited dictionary function.
     predicate dict(a: string)
     {
-        a in ["a", "as"]
+        a == "a" 
+        || a == "as"
+        || a == "the"
     }
 
+    /**
+     * An axiom stating if there exists
+     * at least one word in string `S`,
+     * the result evaluates to true.
+     */
     predicate greedy_a1(S: string)
+    requires |S| > 0
     {
-        greedy_a1'(S, 0)
+        greedy_a1'(S, 0, 1)
     }
 
-    predicate greedy_a1'(S: string, i: nat)
-    decreases |S| - i 
+    predicate greedy_a1'(S: string, i: nat, j: nat)
+    requires 0 <= i < j <= |S|
+    decreases |S|-i , |S|-j
     {
-        forall j {:induction j}:: 0 <= i < j <= |S| 
-            ==> (dict(S[i..j]) || greedy_a1'(S, j))
+        if dict(S[i..j]) then
+            true
+        else if j+1 <= |S| then
+            greedy_a1'(S, i, j+1) 
+        else if i+2 <= |S| then
+            greedy_a1'(S, i+1, i+2) 
+        else false
     }
 
     method Main()
     {
-        var s1, s2, s3, s4, s5 := "a", "as", "aas", "aa", "s";
-        assert s1[0] == 'a';
-        assert |s1| == 1;
-        assert |s3| == 3;
-        assert s5[0] == 's';
-        assert dict(s5) == false;
+        // Positives.
+        var s1, s2, s3, s4 := "a", "as", "aas", "aa";
+        var s6 := "asa";
+        var s7 := "sa";
+
+        // Negatives.
+        var s5 := "s";
+        var s8 := "xx";
+
         assert greedy_a1(s1) == true;
         assert greedy_a1(s2) == true;
-        assert greedy_a1(s5) == false;
         assert greedy_a1(s3) == true;
         assert greedy_a1(s4) == true;
+        assert greedy_a1(s6) == true;
+        assert greedy_a1(s7) == true;
+
+        // This is needed for some reason- might need a lemma?
+        assert dict(s5) == false;
+        assert greedy_a1(s5) == false;
+        assert greedy_a1(s8) == false;
     }
 }
